coq/SimpleForm/Tactics.v
@@ -290,122 +290,38 @@ Ltac crusher_c strength :=
   end;
   finish.
 
-Section SAP.
-  Variables reg_t ext_fn_t: Type.
-Lemma subact_at_pos_refl: forall (x: sact (reg_t:=reg_t) (ext_fn_t:=ext_fn_t)),
-    subact_at_position x [] = Some x.
-Proof.
-  induction x; simpl; intros; reflexivity.
-Qed.
 
-Lemma subact_at_pos_rev_refl: forall (x: sact (reg_t:=reg_t) (ext_fn_t:=ext_fn_t)),
-    subact_at_position x (List.rev []) = Some x.
-Proof.
-  intros; simpl; eapply subact_at_pos_refl.
-Qed.
-
-
-Lemma subact_at_pos_trans:
-  forall (s: sact (reg_t:=reg_t) (ext_fn_t:=ext_fn_t)) p1 s1 p2 s2,
-    subact_at_position s p1 = Some s1 ->
-    subact_at_position s1 p2 = Some s2 ->
-    subact_at_position s (p1 ++ p2) = Some s2.
-Proof.
-  induction s; simpl; intros;
-    repeat destr_in H; inv H; simpl in *; eauto.
-Qed.
-
-Lemma subact_at_pos_unop1:
-  forall (s: @sact reg_t ext_fn_t) pos ufn a,
-    subact_at_position s (List.rev pos) = Some (SUnop ufn a) ->
-    subact_at_position s (List.rev (branch1 :: pos)) = Some a.
-Proof.
-  intros. simpl. erewrite subact_at_pos_trans. 2: eauto. eauto. simpl.
-  apply subact_at_pos_refl.
-Qed.
-
-Lemma subact_at_pos_extcall1:
-  forall (s: @sact reg_t ext_fn_t) pos ufn a,
-    subact_at_position s (List.rev pos) = Some (SExternalCall ufn a) ->
-    subact_at_position s (List.rev (branch1 :: pos)) = Some a.
-Proof.
-  intros. simpl. erewrite subact_at_pos_trans. 2: eauto. eauto. simpl.
-  apply subact_at_pos_refl.
-Qed.
-
-Lemma subact_at_pos_binop1:
-  forall (s: @sact reg_t ext_fn_t) pos ufn a1 a2,
-    subact_at_position s (List.rev pos) = Some (SBinop ufn a1 a2) ->
-    subact_at_position s (List.rev (branch1 :: pos)) = Some a1.
-Proof.
-  intros. simpl. erewrite subact_at_pos_trans. 2: eauto. eauto. simpl.
-  apply subact_at_pos_refl.
-Qed.
-
-Lemma subact_at_pos_binop2:
-  forall (s: @sact reg_t ext_fn_t) pos ufn a1 a2,
-    subact_at_position s (List.rev pos) = Some (SBinop ufn a1 a2) ->
-    subact_at_position s (List.rev (branch2 :: pos)) = Some a2.
-Proof.
-  intros. simpl. erewrite subact_at_pos_trans. 2: eauto. eauto. simpl.
-  apply subact_at_pos_refl.
-Qed.
-
-
-Lemma subact_at_pos_if1:
-  forall (s: @sact reg_t ext_fn_t) pos a1 a2 a3,
-    subact_at_position s (List.rev pos) = Some (SIf a1 a2 a3) ->
-    subact_at_position s (List.rev (branch1 :: pos)) = Some a1.
-Proof.
-  intros. simpl. erewrite subact_at_pos_trans. 2: eauto. eauto. simpl.
-  apply subact_at_pos_refl.
-Qed.
-
-Lemma subact_at_pos_if2:
-  forall (s: @sact reg_t ext_fn_t) pos a1 a2 a3,
-    subact_at_position s (List.rev pos) = Some (SIf a1 a2 a3) ->
-    subact_at_position s (List.rev (branch2 :: pos)) = Some a2.
-Proof.
-  intros. simpl. erewrite subact_at_pos_trans. 2: eauto. eauto. simpl.
-  apply subact_at_pos_refl.
-Qed.
-
-Lemma subact_at_pos_if3:
-  forall (s: @sact reg_t ext_fn_t) pos a1 a2 a3,
-    subact_at_position s (List.rev pos) = Some (SIf a1 a2 a3) ->
-    subact_at_position s (List.rev (branch3 :: pos)) = Some a3.
-Proof.
-  intros. simpl. erewrite subact_at_pos_trans. 2: eauto. eauto. simpl.
-  apply subact_at_pos_refl.
-Qed.
 
 
 Ltac search_subterm needle haystack pos orig_haystack Ppos :=
   match haystack with
   | ?x => match needle with
-            x => eval vm_compute in
-              (existT _ [pos] (Forall_cons pos Ppos (@Forall_nil _ (fun v => subact_at_position orig_haystack (List.rev v) = Some needle))))
+            x => let res := constr:(ssprop_one pos needle orig_haystack Ppos) in
+                 eval vm_compute in res
           end
-  | SVar ?x => eval vm_compute in
-      (existT _ _ (@Forall_nil _ (fun v => subact_at_position orig_haystack (List.rev v) = Some needle)))
-  | SConst ?x =>  eval vm_compute in
-      (existT _ _ (@Forall_nil _ (fun v => subact_at_position orig_haystack (List.rev v) = Some needle)))
-  | SReg ?x =>  eval vm_compute in
-      (existT _ _ (@Forall_nil _ (fun v => subact_at_position orig_haystack (List.rev v) = Some needle)))
+  | SVar ?x => let res := constr:(ssprop_nil needle orig_haystack pos) in
+                 eval vm_compute in res
+  | SConst ?x => let res := constr:(ssprop_nil needle orig_haystack pos) in
+                 eval vm_compute in res
+  | SReg ?x => let res := constr:(ssprop_nil needle orig_haystack pos) in
+                 eval vm_compute in res
   | SUnop ?ufn ?a =>
-      search_subterm needle a (Direction.branch1 :: pos) orig_haystack (subact_at_pos_unop1 _ _ _ _ Ppos)
+      let p := search_subterm needle a (Direction.branch1 :: pos) orig_haystack (subact_at_pos_unop1 _ _ _ _ Ppos) in
+      eval vm_compute in (sprop_unop needle pos _ p)
   | SExternalCall ?ufn ?a =>
-      search_subterm needle a (Direction.branch1 :: pos) orig_haystack (subact_at_pos_extcall1 _ _ _ _ Ppos)
+      let p := search_subterm needle a (Direction.branch1 :: pos) orig_haystack (subact_at_pos_extcall1 _ _ _ _ Ppos) in
+      eval vm_compute in (sprop_unop needle pos _ p)
   | SBinop ?ufn ?a ?b =>
       let p1 := search_subterm needle a (Direction.branch1 :: pos) orig_haystack (subact_at_pos_binop1 _ _ _ _ _ Ppos) in
       let p2 := search_subterm needle b (Direction.branch2 :: pos) orig_haystack (subact_at_pos_binop2 _ _ _ _ _ Ppos) in
-      eval vm_compute in (existT _ _ (proj2 (@Forall_app _ _ _ _) (conj (projT2 p1) (projT2 p2))))
+      eval vm_compute in
+        (sprop_binop needle pos _ p1 p2)
   | SIf ?a ?b ?c =>
       let p1 := search_subterm needle a (Direction.branch1 :: pos) orig_haystack (subact_at_pos_if1 _ _ _ _ _ Ppos) in
       let p2 := search_subterm needle b (Direction.branch2 :: pos) orig_haystack (subact_at_pos_if2 _ _ _ _ _ Ppos) in
       let p3 := search_subterm needle c (Direction.branch3 :: pos) orig_haystack (subact_at_pos_if3 _ _ _ _ _ Ppos) in
       eval vm_compute in
-        (existT _ _ (proj2 (@Forall_app _ _ _ _) (conj (projT2 p1) (proj2 (@Forall_app _ _ _ _) (conj (projT2 p2) (projT2 p3))))))
+        (sprop_if needle pos _ p1 p2 p3)
   end.
 
 
@@ -415,112 +331,83 @@ Ltac ssearch needle haystack :=
     search_subterm needle hs ([]: list Direction.direction) hs (subact_at_pos_rev_refl hs) in
   res.
 
-Definition ptree_forall {A: Type} (P: positive -> A -> Prop) (t: Maps.PTree.t A) :=
-  forall k v, Maps.PTree.get k t = Some v -> P k v.
 
-Lemma ptree_set_prop {A: Type} (t: Maps.PTree.t A) P
-  (FA: ptree_forall P t)
-  k v
-  (PKV: P k v):
-  ptree_forall P (Maps.PTree.set k v t).
-Proof.
-  unfold ptree_forall in *.
+Goal forall (reg_t ext_fn_t: Type) (uext:ext_fn_t), False.
   intros.
-  rewrite Maps.PTree.gsspec in H. destr_in H; eauto. inv H. auto.
-Qed.
+  let l := ssearch (SConst (reg_t:=reg_t) (ext_fn_t:=ext_fn_t) (Bits [true]))
+             (SConst (Bits [true]) : (@sact reg_t ext_fn_t)) in
+  idtac l;
+  let t := (type of l) in idtac t.
 
-Lemma ptree_forall_empty {A: Type} P:
-  ptree_forall P (Maps.PTree.empty A).
-Proof.
-  unfold ptree_forall. intros. rewrite Maps.PTree.gempty in H. congruence.
-Qed.
+  let l := ssearch (SConst (reg_t:=reg_t) (ext_fn_t:=ext_fn_t) (Bits [true]))
+             (SVar 12%positive : ((@sact reg_t ext_fn_t))) in
+  idtac l;
+  let t := (type of l) in idtac t.
+
+  let l := ssearch (SConst (reg_t:=reg_t) (ext_fn_t:=ext_fn_t) (Bits [true]))
+             (SUnop (PrimUntyped.UBits1 PrimUntyped.UNot) (SVar 12%positive : ((@sact reg_t ext_fn_t)))) in
+  idtac l;
+  let t := (type of l) in idtac t.
+
+  let l := ssearch (SConst (reg_t:=reg_t) (ext_fn_t:=ext_fn_t) (Bits [true]))
+             (SBinop (PrimUntyped.UBits2 PrimUntyped.UAnd)
+                (SConst (reg_t:=reg_t) (ext_fn_t:=ext_fn_t) (Bits [true]))
+                (SVar 12%positive : ((@sact reg_t ext_fn_t)))) in
+  let t := (type of l) in idtac t.
+
+
+  let l := ssearch (SConst (reg_t:=reg_t) (ext_fn_t:=ext_fn_t) (Bits [true]))
+             (SExternalCall uext (SIf
+                       (SUnop (PrimUntyped.UBits1 PrimUntyped.UNot) (SBinop (PrimUntyped.UBits2 PrimUntyped.UAnd)
+                   (SConst (reg_t:=reg_t) (ext_fn_t:=ext_fn_t) (Bits [true]))
+                   (SVar 12%positive : ((@sact reg_t ext_fn_t)))))
+                (SConst (Bits [true]))
+                (SConst (Bits [false]))))
+               in
+  let t := (type of l) in idtac t.
+
+
+Abort.
 
 Ltac ssearch_in_elems needle l :=
   lazymatch l with
-  | [] => eval vm_compute in (existT (A:=list (positive * list position))
-                                (fun v =>
-                                   Forall2 (fun '(k, (t, a)) '(k1, ps) =>
-                                              k = k1 /\
-                                              Forall (fun p => subact_at_position a (rev p) = Some needle) ps
-                                     ) l v
-                                ) _ (Forall2_nil _)
-                             )
+  | [] => eval vm_compute in (ssearch_in_elemsT_nil needle)
   | (?kk, (?tt, ?x))::?r =>
       let ps := ssearch needle x in
       let pss := ssearch_in_elems needle r in
       eval vm_compute in
-        (existT (A:=list (positive * list position))
-           _ _ (@Forall2_cons _ _ (fun '(k, (t, a)) '(k1,Ps) =>
-                                     k = k1 /\
-                                       Forall (fun p => subact_at_position a (rev p) = Some needle) Ps
-                                     ) (kk,(tt,x)) (kk,(projT1 ps)) _ _ (conj eq_refl (projT2 ps)) (projT2 pss)))
-  end.
-
-Fixpoint ptree_of_elements {A: Type} (l: list (positive * A)) :=
-  match l with
-    [] => Maps.PTree.empty A
-  | (k,v)::r => Maps.PTree.set k v (ptree_of_elements r)
+        (ssearch_in_elemsT_cons needle r kk tt _ _ pss ps)
   end.
 
 
-Lemma forall2_elems:
-  forall {A B: Type}
-         (l1: list (positive * A))
-         (l2: list (positive * B)) P,
-    Forall2 (fun '(k, a) '(k1,v) => k = k1 /\ P a v) l1 l2 ->
-    NoDup (List.map fst l1) ->
-    let res := ptree_of_elements l2 in
-    forall k ps a,
-      In (k, a) l1 ->
-      Maps.PTree.get k res = Some ps ->
-      P a ps.
-Proof.
-  induction 1; simpl; intros; eauto. easy.
-  destr_in H3.
-  rewrite Maps.PTree.gsspec in H3.
-  destruct x. destruct H. subst. simpl in H1. inv H1.
-  destr_in H3.
-  - inv H3. destruct H2 as [C|C]. inv C. auto.
-    elim H6. change p with (fst (p, a)). apply in_map. auto.
-  - destruct H2. inv H. congruence.
-    eauto.
-Qed.
-
-
-Lemma forall2_elems':
-  forall {A B: Type}
-         (l1: Maps.PTree.t A)
-         (l2: list (positive * B)) P,
-    Forall2 (fun '(k, a) '(k1,v) => k = k1 /\ P a v) (Maps.PTree.elements l1) l2 ->
-    let res := ptree_of_elements l2 in
-    forall k ps a,
-      Maps.PTree.get k l1 = Some a ->
-      Maps.PTree.get k res = Some ps ->
-      P a ps.
-Proof.
+Goal forall (reg_t ext_fn_t: Type) (uext:ext_fn_t), False.
   intros.
-  eapply forall2_elems; eauto.
-  apply Maps.PTree.elements_keys_norepet.
-  apply Maps.PTree.elements_correct; auto.
-Qed.
+    Import PrimUntyped.
 
+    set (vars :=
+           Maps.PTree.set 1%positive (bits_t 1, SConst (reg_t:=reg_t) (ext_fn_t:=ext_fn_t) (Bits [true]))
+             (Maps.PTree.set 2%positive (bits_t 1, SUnop (UBits1 UNot) (SConst (reg_t:=reg_t) (ext_fn_t:=ext_fn_t) (Bits [true])))
+                (Maps.PTree.set 3%positive (bits_t 1, SBinop (UBits2 UAnd)
+           (SConst (reg_t:=reg_t) (ext_fn_t:=ext_fn_t) (Bits [true]))
+           (SConst (reg_t:=reg_t) (ext_fn_t:=ext_fn_t) (Bits [true]))
+                   ) (Maps.PTree.set 4%positive (bits_t 1,
+(SExternalCall uext (SIf
+                       (SUnop (UBits1 UNot) (SBinop (PrimUntyped.UBits2 PrimUntyped.UAnd)
+                   (SConst (reg_t:=reg_t) (ext_fn_t:=ext_fn_t) (Bits [true]))
+                   (SVar 12%positive : ((@sact reg_t ext_fn_t)))))
+                (SConst (Bits [true]))
+                (SConst (Bits [false]))))
+                        ) (Maps.PTree.empty _)))
+             )
+        ).
 
-Lemma forall2_elems'':
-  forall {A B C: Type}
-         (l1: Maps.PTree.t (C * A))
-         (l2: list (positive * B)) P,
-    Forall2 (fun '(k, (t, a)) '(k1,v) => k = k1 /\ P a v) (Maps.PTree.elements l1) l2 ->
-    let res := ptree_of_elements l2 in
-    forall k ps t a,
-      Maps.PTree.get k l1 = Some (t, a) ->
-      Maps.PTree.get k res = Some ps ->
-      P a ps.
-Proof.
-  intros.
-  eapply forall2_elems' with (P0:=fun '(t,a) v => P a v) in H0. eauto.
-  2: eauto.
-  eapply Forall2_impl. eauto. simpl. intros. destruct x. destruct p0,y. destruct H4. subst. split; auto.
-Qed.
+    Set Ltac Backtrace.
+
+    let vars := eval vm_compute in (Maps.PTree.elements vars) in
+      let res := ssearch_in_elems (SConst (reg_t:=reg_t) (ext_fn_t:=ext_fn_t) (Bits [true]))
+                   vars in
+      let t := type of res in idtac t.
+Abort.
 
 
 Ltac ssearch_in_vars needle t :=
@@ -532,39 +419,53 @@ Ltac ssearch_in_vars needle t :=
           let H := fresh in
           assert (H: Forall2 (fun '(k, (ty,a)) '(k1,ps) =>
                              k = k1 /\
-                               (fun '(_,a) ps => Forall (fun p => subact_at_position a (rev p) = Some needle) ps) (ty,a) ps
+                               (fun '(_,a) ps =>
+                                  search_subterm_propP needle a [] ps) (ty,a) ps
                     )
                        (Maps.PTree.elements t) x) by (exact P);
           let H2 := fresh in
           assert (H2 := forall2_elems'' _ _ _ H); clear H.
 
 
-Goal False.
+Goal forall (reg_t ext_fn_t: Type) (uext: ext_fn_t), False.
+  intros.
     set (k0:= true: bool).
     Import PrimUntyped.
 
-    set (vars :=
+        set (vars :=
            Maps.PTree.set 1%positive (bits_t 1, SConst (reg_t:=reg_t) (ext_fn_t:=ext_fn_t) (Bits [true]))
              (Maps.PTree.set 2%positive (bits_t 1, SUnop (UBits1 UNot) (SConst (reg_t:=reg_t) (ext_fn_t:=ext_fn_t) (Bits [true])))
                 (Maps.PTree.set 3%positive (bits_t 1, SBinop (UBits2 UAnd)
            (SConst (reg_t:=reg_t) (ext_fn_t:=ext_fn_t) (Bits [true]))
            (SConst (reg_t:=reg_t) (ext_fn_t:=ext_fn_t) (Bits [true]))
-                   ) (Maps.PTree.empty _))
+                   ) (Maps.PTree.set 4%positive (bits_t 1,
+(SExternalCall uext (SIf
+                (SBinop (PrimUntyped.UBits2 PrimUntyped.UAnd)
+                   (SConst (reg_t:=reg_t) (ext_fn_t:=ext_fn_t) (Bits [true]))
+                   (SVar 12%positive : ((@sact reg_t ext_fn_t))))
+                (SConst (Bits [true]))
+                (SConst (Bits [false]))))
+                        ) (Maps.PTree.empty _)))
              )
         ).
 
     Set Ltac Backtrace.
 
+    (* let vars := eval vm_compute in (Maps.PTree.elements vars) in *)
+    (*   let res := ssearch_in_elems (SConst (reg_t:=reg_t) (ext_fn_t:=ext_fn_t) (Bits [true])) *)
+    (*           vars in idtac res. *)
+
+
     ssearch_in_vars (SConst (reg_t:=reg_t) (ext_fn_t:=ext_fn_t) (Bits [true]))
               vars.
 
     let l := ssearch (SConst (reg_t:=reg_t) (ext_fn_t:=ext_fn_t) (Bits [true]))
-               (SConst (Bits [true]) : (@sact reg_t ext_fn_t)) in idtac l.
+               (SConst (Bits [true]) : ((@sact reg_t ext_fn_t))) in idtac l.
 
-    let l :=
-      ssearch_in_elems (SConst (reg_t:=reg_t) (ext_fn_t:=ext_fn_t) (Bits [true]))
-                       ([(1%positive, (bits_t 1, SConst (Bits [true])))] : list (prod positive (prod type (@sact reg_t ext_fn_t))))
-    in idtac l.
+    (* let l := *)
+    (*   ssearch_in_elems (SConst (reg_t:=reg_t) (ext_fn_t:=ext_fn_t) (Bits [true])) *)
+    (*                    ([(1%positive, (bits_t 1, SConst (Bits [true])))] : list (prod positive (prod type ((@sact reg_t ext_fn_t))))) *)
+    (* in idtac l. *)
 
 
     set (hs := (SConst (reg_t:=reg_t) (ext_fn_t:=ext_fn_t) (Bits [true]))).
@@ -593,4 +494,3 @@ Goal False.
     idtac x.
 Abort.
 
-End SAP.
